Find the equations of tangent line to the curve:

$$3(y-2)^2 - (x-1)^2=3$$

if the tangent line also passes trough the point (0,2).

$$3(y-2)^2-x^2+2x-1=3$$

$$(y-2)^2=\frac{1}{3}(x^2-2x+4)$$

$$y-2=\frac{1}{\sqrt{3}}\sqrt{x^2-2x+4}$$

$$y=\frac{1}{\sqrt{3}}\sqrt{x^2-2x+4} + 2$$

$$y= \frac{1}{3} (6 + \sqrt{3} \sqrt{4 - 2 x + x^2}) $$

The derivative:

$$\frac{dy}{dx} = \frac{-1 + x}{\sqrt{3} \sqrt{4 - 2 x + x^2}}$$

The tangent line:

$$y = mx + b \quad and \quad (0,2) => \quad b = 2$$

You can think of a line in the form y=mx+b, where m = (y2-y1)/(x2-x1)

You could use m=(y2-2)/(x2-0). 

You also know that (x2,y2) satisfies the original curve equation, and that m also equals the derivative you computed.

$$\frac{-1 + x}{\sqrt{3} \sqrt{4 - 2 x + x^2}}=\frac{\frac{1}{3} (6 + \sqrt{3} \sqrt{4 - 2 x + x^2}) -2}{x}$$
